fe25519/bvdsl/fe25519_sub.v
@@ -1,7 +1,7 @@
 
 From Coq Require Import ZArith.
 From mathcomp Require Import ssreflect ssrbool ssrnat seq.
-From Common Require Import Bits.
+From Common Require Import Var Bits.
 From mQhasm Require Import bvDSL bvVerify Options.
 
 Set Implicit Arguments.
